src/spl/Syntactic.v
@@ -122,13 +122,13 @@ Section CheckAtom.
         intros [ | | | | | | | | i0 n0 n1| n i0| n i0] i Heq H; try discriminate; simpl;
       unfold apply_unop; rewrite (check_hatom_correct _ _ H); 
       unfold interp_hatom; rewrite (t_interp_wf _ _ _ Hwf Hd i2), Heq; simpl; 
-      unfold apply_unop; destruct (t_interp t_i t_func t_atom .[ i]) as [A v]; 
+      unfold apply_unop; destruct ((t_interp t_i t_func t_atom) .[ i]) as [A v]; 
       destruct (Typ.cast A Typ.Tpositive) as [k| ]; auto.
       case_eq (get_atom i1); try discriminate;
         intros [ | | | | | | | | i0 n0 n1| n i0| n i0] i Heq H; try discriminate; simpl; 
       unfold apply_unop. rewrite <- (check_hatom_correct _ _ H); 
       unfold interp_hatom; rewrite (t_interp_wf _ _ _ Hwf Hd i1), Heq; simpl; 
-      unfold apply_unop; destruct (t_interp t_i t_func t_atom .[ i]) as [A v]; 
+      unfold apply_unop; destruct ((t_interp t_i t_func t_atom) .[ i]) as [A v]; 
       destruct (Typ.cast A Typ.Tpositive) as [k| ]; auto.
 
       intros n m n1 m2. simpl. unfold is_true. rewrite !andb_true_iff, beq_nat_true_iff, N.eqb_eq. intros [[-> ->] H]. rewrite (check_hatom_correct _ _ H); auto.
